horrible, but working proof

TAPLFormalization/SemanticsTheorems.lean
@@ -1,15 +1,128 @@
 import TAPLFormalization.Semantics
 
-theorem smallStepDeterministic : (t₁ ~> t₂) → (t₁ ~> t₃) → (t₂ = t₃) := by
-  sorry
+theorem headSmallStep_deterministic : HeadSmallStep t t₁ → HeadSmallStep t t₂ → (t₁ = t₂) := by
+  intro h_st₁ h_st₂
+  cases h_st₁ <;> cases h_st₂ <;> rfl
+
+inductive isRedex : Term → Prop
+  | ifTrue : isRedex (.ifThenElse (.value .trueV) t₂ t₃)
+  | ifFalse : isRedex (.ifThenElse (.value .falseV) t₂ t₃)
+  | predZero : isRedex (.pred (.value (.nv .zero)))
+  | predSucc : isRedex (.pred (.succ (.value (.nv n))))
+  | isZeroZero : isRedex (.isZero (.value (.nv .zero)))
+  | isZeroSucc : isRedex (.isZero (.value (.nv (.succ n))))
+
+lemma isRedex_iff_can_headSmallStep : (∃ t', HeadSmallStep t t') ↔ isRedex t := by
+  apply Iff.intro
+  · rintro ⟨t', h_st⟩
+    cases h_st <;> try constructor
+  · intro t_redex
+    cases t_redex with
+    | ifTrue =>
+      rename_i t₂ t₃
+      exists t₂
+      constructor
+    | ifFalse =>
+      rename_i t₂ t₃
+      exists t₃
+      constructor
+    | predZero =>
+      exists .value (.nv .zero)
+      constructor
+    | predSucc =>
+      rename_i n
+      exists .value (.nv n)
+      constructor
+    | isZeroZero =>
+      exists .value .trueV
+      constructor
+    | isZeroSucc =>
+      exists .value .falseV
+      constructor
+
+def isDecomposition (t : Term) (ctx : Ctx) (t' : Term) := isRedex t' ∧ t = ctx.fill t'
+
+lemma decomposition_unique_with_hole (t : Term) : isDecomposition t ctx t₁ → isRedex t → ctx = .hole ∧ t₁ = t := by
+  rintro ⟨t₁_redex, t_eq₁⟩ t_redex
+  cases t_redex <;> cases ctx <;> simp [Ctx.fill] at t_eq₁ <;> try (
+    constructor
+    · rfl
+    · try exact t_eq₁
+      try exact Eq.symm t_eq₁
+  )
+  all_goals rename Ctx => ctx'
+  all_goals try let ⟨t_eq₁, _, _⟩ := t_eq₁
+  all_goals cases ctx' <;> simp [Ctx.fill] at t_eq₁
+  all_goals try (
+    rw [← t_eq₁] at t₁_redex
+    cases t₁_redex
+  )
+  rename_i ctx''
+  cases ctx'' <;> simp [Ctx.fill] at t_eq₁
+  rw [← t_eq₁] at t₁_redex
+  cases t₁_redex
+
+lemma decomposition_unique (t : Term) : isDecomposition t ctx₁ t₁ → isDecomposition t ctx₂ t₂
+  → ctx₁ = ctx₂ ∧ t₁ = t₂ := by
+  rintro ⟨t₁_redex, t_eq₁⟩ ⟨t₂_redex, t_eq₂⟩
+  induction ctx₂ generalizing t ctx₁
+  case hole =>
+    rw [Ctx.fill] at t_eq₂
+    rw [t_eq₂] at t_eq₁ t_eq₂
+    exact decomposition_unique_with_hole t₂ ⟨t₁_redex, t_eq₁⟩ t₂_redex
+  case ifThenElse ctx₁' t₁ t₂ ih =>
+    rw [t_eq₁] at t_eq₂
+    cases ctx₁ <;> (
+      simp only [Ctx.fill] at t_eq₂
+      try cases t_eq₂
+    )
+    · rw [Ctx.fill] at t_eq₁
+      rw [← t_eq₁] at t₁_redex
+      rw [← Ctx.fill] at t_eq₁
+      let ⟨ctx_eq, t_eq⟩ := decomposition_unique_with_hole t ⟨t₂_redex, t_eq₁⟩ t₁_redex
+      cases ctx_eq
+    · rename_i t₂' t₁' ctx₂' t₁_copy t₂_copy
+      generalize h₁ : Ctx.fill t₁' ctx₁' = fill₁
+      generalize h₂ : Ctx.fill t₂' ctx₂' = fill₂
+      rw [h₁, h₂] at t_eq₂
+      cases t_eq₂
+      let ⟨ctx_eq, t_eq⟩ := ih fill₁ (Eq.symm h₂) (Eq.symm h₁)
+      constructor <;> simp only [ctx_eq, t_eq]
+  all_goals (
+    rename_i ctx₁' ih
+    rw [t_eq₁] at t_eq₂
+    cases ctx₁ <;> (
+      simp only [Ctx.fill] at t_eq₂
+      try cases t_eq₂
+    )
+    · rw [Ctx.fill] at t_eq₁
+      rw [← t_eq₁] at t₁_redex
+      rw [← Ctx.fill] at t_eq₁
+      let ⟨ctx_eq, t_eq⟩ := decomposition_unique_with_hole t ⟨t₂_redex, t_eq₁⟩ t₁_redex
+      cases ctx_eq
+    · rename_i ctx₂'
+      generalize h₁ : Ctx.fill t₁ ctx₂' = fill₁
+      generalize h₂ : Ctx.fill t₂ ctx₁' = fill₂
+      rw [h₁, h₂] at t_eq₂
+      cases t_eq₂
+      let ⟨ctx_eq, t_eq⟩ := ih fill₁ (Eq.symm h₁) (Eq.symm h₂)
+      constructor <;> simp only [ctx_eq, t_eq]
+  )
+
+theorem smallStep_deterministic : (t ~> t₁) → (t ~> t₂) → (t₁ = t₂) := by
+  rintro ⟨ctx₁, t_eq₁, t₁_eq, h_st₁⟩ ⟨ctx₂, t_eq₂, t₂_eq, h_st₂⟩
+  rename_i t_redex₁ t₁_redex t_redex₂ t₂_redex
+  let t_redex₁_is_redex := isRedex_iff_can_headSmallStep.mp ⟨_, h_st₁⟩
+  let t_redex₂_is_redex := isRedex_iff_can_headSmallStep.mp ⟨_, h_st₂⟩
+  let ⟨ctx_eq, t_redex_eq⟩ := decomposition_unique t ⟨t_redex₁_is_redex, t_eq₁⟩ ⟨t_redex₂_is_redex, t_eq₂⟩
+  rw [t_redex_eq] at h_st₁
+  let t₁₂_redex_eq := headSmallStep_deterministic h_st₁ h_st₂
+  rw [t₁_eq, t₂_eq, ctx_eq, t₁₂_redex_eq]
 
 def isNF (t : Term) := ∀ (t' : Term), ¬(t ~> t')
 
 inductive isValue : Term → Prop where
   | value v : isValue (.value v)
-
-theorem isNF_iff_isValue : ∀ (t : Term), isNF t ↔ isValue t := by
-  sorry
 
 theorem NF_unique : (t ~>* u) → (t ~>* u') → isNF u → isNF u' → u = u' := by
   sorry
